\chapter{Appendix to ``Difference-in-Differences with Spatial Spillovers''}

% ------------------------------------------------------------------------------
\section{Proofs}
\label{sec:spillover-proofs}
% ------------------------------------------------------------------------------

% ------------------------------------------------------------------------------
\subsection{Proof of Proposition \ref{prop:bias}}
% ------------------------------------------------------------------------------

\begin{align*}
    &\underbrace{\expec{Y_{i1} - Y_{i0} \mid D_i = 1 } - \expec{Y_{i1} - Y_{i0} \mid D_i = 0 }}_{\text{Difference-in-Differences}} \\
    &= \expec{Y_{i1}(1, h_i(\bm{D})) - Y_{i0}(0, \bm{0})  \mid D_i = 1 } - \expec{Y_{i1}(0, h_i(\bm{D})) - Y_{i0}(0, \bm{0}) \mid D_i = 0 } \\
    % &= \expec{Y_{i1}(1, h_i(\bm{D})) - Y_{i0}(0, \bm{0})  \mid D_i = 1 } \\
    % &\quad\quad - \expec{Y_{i1}(0, h_i(\bm{D})) + Y_{i1}(0, \bm{0}) - Y_{i1}(0, \bm{0}) - Y_{i0}(0, \bm{0}) \mid D_i = 0 } \\
    &= \expec{Y_{i1}(1, h_i(\bm{D})) - Y_{i0}(0, \bm{0})  \mid D_i = 1 } - \expec{Y_{i1}(0, \bm{0}) - Y_{i0}(0, \bm{0}) \mid D_i = 0} \\ 
    &\quad\quad - \expec{Y_{i1}(0, h_i(\bm{D})) - Y_{i1}(0, \bm{0})\mid D_i = 0} \\ 
    &= \expec{Y_{i1}(1, h_i(\bm{D})) - Y_{i0}(0, \bm{0})  \mid D_i = 1 } - \expec{Y_{i1}(0, \bm{0}) - Y_{i0}(0, \bm{0}) \mid D_i = 1} \\
    &\quad\quad - \expec{Y_{i1}(0, h_i(\bm{D})) - Y_{i1}(0, \bm{0})\mid D_i = 0} \\  
    % &= \expec{Y_{i1}(1, h_i(\bm{D})) - Y_{i0}(0, \bm{0}) - Y_{i1}(0, \bm{0}) + Y_{i0}(0, \bm{0})\mid D_i = 1 } \\
    % &\quad\quad - \expec{Y_{i1}(0, h_i(\bm{D})) - Y_{i1}(0, \bm{0})\mid D_i = 0}\\
    &= \expec{Y_{i1}(1, h_i(\bm{D})) - Y_{i1}(0, \bm{0}) \mid D_i = 1 } - \expec{Y_{i1}(0, h_i(\bm{D})) - Y_{i1}(0, \bm{0})\mid D_i = 0} \\
    &\equiv \tau_{\text{total}} - \tau_{\text{spill}}(0), 
\end{align*}
where the first equality comes from the potential outcomes and the \nameref{assumption:no-anticipation} assumption, the second from adding and subtracting terms, the third equality follows from the \nameref{assumption:parallel} assumption, and the final equality follows from the definitions of total and spillover effects.

% ------------------------------------------------------------------------------
\subsection{Proof of Proposition \ref{prop:total_effect}}
% ------------------------------------------------------------------------------

\begin{align*}
    &\expec{Y_{i1} - Y_{i0} \ \mid \ D_i = 1} - \expec{Y_{i1} - Y_{i0} \ \mid \ D_i = 0, S_i =0} \\
    &\quad\quad= \expec{Y_{i1}(1, h_i(\bm{D})) - Y_{i0}(0, \bm{0}) \ \mid \ D_i = 1} - \expec{Y_{i1}(0, \bm{0}) - Y_{i0}(0, \bm{0}) \ \mid \ D_i = 0, S_i =0} \\
    &\quad\quad= \expec{Y_{i1}(1, h_i(\bm{D})) - Y_{i0}(0, \bm{0}) \ \mid \ D_i = 1} - \expec{Y_{i1}(0, \bm{0}) - Y_{i0}(0, \bm{0}) \ \mid \ D_i = 1} \\
    &\quad\quad= \expec{Y_{i1}(1, h_i(\bm{D})) - Y_{i0}(0, \bm{0}) - Y_{i1}(0, \bm{0}) + Y_{i0}(0, \bm{0}) \ \mid \ D_i = 1} \\
    &\quad\quad= \expec{Y_{i1}(1, h_i(\bm{D})) - Y_{i1}(0, \bm{0}) \ \mid \ D_i = 1} \\
    &\quad\quad\equiv \tau_{\text{total}},
\end{align*}
where the first equality comes from the fact that $S_i = 0$ implies $h_i(\bm{D}) = 0$, the second equality from parallel trends assumption (\ref{assumption:parallel-mod}), and the last by definition of the total effect.



% ------------------------------------------------------------------------------
\subsection{Identification of Imputation Estimator}\label{sec:identification_imputation}
% ------------------------------------------------------------------------------

This section will give identification arguments for the total effect and spillover effects. First, note under \nameref{assumption:parallel_staggered}, we have 
\begin{align*}
  \expec{Y_{it}(d_{it}, h_i(\bm{D}_t)) - \mu_i - \lambda_t \ | \ d_{it} = 1} 
  &= \expec{\tau_{it}(d_{it}, h_i(\bm{D}_t)) + \varepsilon_{it} \ | \ d_{it} = 1} \\
  &= \expec{\tau_{it}(d_{it}, h_i(\bm{D}_t)) \ | \ d_{it} = 1} \\
  &= \tau_{total}.
\end{align*}
In the first stage, we estimate $\mu_i$ and $\lambda_t$ using observations with $d_{it}$ and $S_{it} = 0$. Unbiasedness/consistency follows from \nameref{assumption:local} and \nameref{assumption:no-anticipation_staggered} and the arguments of the appendix of \citet{Gardner_2021}.

A similar argument follows for spillover effects. Again, assuming \nameref{assumption:parallel_staggered}, we have 
\begin{align*}
  \expec{Y_{it}(d_{it}, h_i(\bm{D}_t)) - \mu_i - \lambda_t \ | \ d_{it} = 0, S_{it} = 1} 
  &= \expec{\tau_{it}(d_{it}, h_i(\bm{D}_t)) + \varepsilon_{it} \ | \ d_{it} = 0, S_{it} = 0} \\
  &= \expec{\tau_{it}(d_{it}, h_i(\bm{D}_t)) \ | \ d_{it} = 0, S_{it} = 1}.
\end{align*}
\vspace*{-5mm}
